more work on impl

Impl/CommitterInitModel.i.dfy
@@ -96,4 +96,207 @@ module CommitterInitModel {
 
     }
   }
+
+  function {:opaque} PageInSuperblockResp(k: Constants, cm: CM, io: IO, which: uint64) : (cm' : CM)
+  requires diskOp(io).RespReadOp?
+  requires ValidDiskOp(diskOp(io))
+  requires which == 0 || which == 1
+  requires which == 0 ==> ValidSuperblock1Location(
+      LocOfRespRead(diskOp(io).respRead))
+  requires which == 1 ==> ValidSuperblock2Location(
+      LocOfRespRead(diskOp(io).respRead))
+  {
+    if cm.status.StatusLoadingSuperblock? then (
+      var (id, sector) := ReadSector(io);
+      var sup := (
+        if sector.Some? &&
+            JournalCache.WFSuperblock(sector.value.superblock) then
+          JournalCache.SuperblockSuccess(sector.value.superblock)
+        else
+          JournalCache.SuperblockCorruption
+      );
+      if which == 0 then (
+        if cm.superblock1Read == Some(id) then 
+          cm.(superblock1Read := None)
+            .(superblock1 := sup)
+        else
+          cm
+      ) else (
+        if cm.superblock2Read == Some(id) then 
+          cm.(superblock2Read := None)
+            .(superblock2 := sup)
+        else
+          cm
+      )
+    ) else (
+      cm
+    )
+  }
+
+  lemma {:opaque} PageInSuperblockRespCorrect(k: Constants, cm: CM, io: IO, which: uint64)
+  requires PageInSuperblockResp.requires(k, cm, io, which)
+  requires CommitterModel.WF(cm)
+  ensures var cm' := PageInSuperblockResp(k, cm, io, which);
+    && CommitterModel.WF(cm')
+    && ValidDiskOp(diskOp(io))
+    && JournalCache.Next(Ik(k).jc,
+        CommitterModel.I(cm),
+        CommitterModel.I(cm'),
+        IDiskOp(diskOp(io)).jdop,
+        JournalInternalOp)
+  {
+    reveal_PageInSuperblockResp();
+    var cm' := PageInSuperblockResp(k, cm, io, which);
+    if cm.status.StatusLoadingSuperblock?
+    {
+      var (id, sector) := ReadSector(io);
+      ReadSectorCorrect(io);
+      var sup := (
+        if sector.Some? &&
+            JournalCache.WFSuperblock(sector.value.superblock) then
+          JournalCache.SuperblockSuccess(sector.value.superblock)
+        else
+          JournalCache.SuperblockCorruption
+      );
+
+      var dop := IDiskOp(diskOp(io)).jdop;
+      assert dop.superblock.Some? ==> sector.Some?;
+      assert sector.Some? ==> dop.superblock.Some?;
+      assert (dop.superblock.Some? && JournalCache.WFSuperblock(dop.superblock.value))
+          == (sector.Some? &&
+            JournalCache.WFSuperblock(sector.value.superblock));
+      //assert sector.value.superblock == diskOp(io).superblock.value;
+
+      if (
+        || (which == 0 && cm.superblock1Read == Some(id))
+        || (which == 1 && cm.superblock2Read == Some(id))
+       )
+      {
+        if which == 0 {
+          assert CommitterModel.I(cm').outstandingSuperblock1Read == None;
+          assert CommitterModel.I(cm').superblock1 == sup;
+          assert CommitterModel.I(cm') == CommitterModel.I(cm)
+              .(outstandingSuperblock1Read := None)
+              .(superblock1 := sup);
+        } else {
+          assert CommitterModel.I(cm').outstandingSuperblock2Read == None;
+          assert CommitterModel.I(cm').superblock2 == sup;
+          assert CommitterModel.I(cm') == CommitterModel.I(cm)
+            .(outstandingSuperblock2Read := None)
+            .(superblock2 := sup);
+        }
+        assert JournalCache.PageInSuperblockResp(Ik(k).jc,
+            CommitterModel.I(cm),
+            CommitterModel.I(cm'),
+            IDiskOp(diskOp(io)).jdop,
+            JournalInternalOp, which as int);
+        assert JournalCache.NextStep(Ik(k).jc,
+            CommitterModel.I(cm),
+            CommitterModel.I(cm'),
+            IDiskOp(diskOp(io)).jdop,
+            JournalInternalOp,
+            JournalCache.PageInSuperblockRespStep(which as int));
+      } else {
+        assert JournalCache.NoOp(Ik(k).jc,
+            CommitterModel.I(cm),
+            CommitterModel.I(cm'),
+            IDiskOp(diskOp(io)).jdop,
+            JournalInternalOp);
+        assert JournalCache.NextStep(Ik(k).jc,
+            CommitterModel.I(cm),
+            CommitterModel.I(cm'),
+            IDiskOp(diskOp(io)).jdop,
+            JournalInternalOp,
+            JournalCache.NoOpStep);
+      }
+    } else {
+      assert JournalCache.NoOp(Ik(k).jc,
+          CommitterModel.I(cm),
+          CommitterModel.I(cm'),
+          IDiskOp(diskOp(io)).jdop,
+          JournalInternalOp);
+      assert JournalCache.NextStep(Ik(k).jc,
+          CommitterModel.I(cm),
+          CommitterModel.I(cm'),
+          IDiskOp(diskOp(io)).jdop,
+          JournalInternalOp,
+          JournalCache.NoOpStep);
+    }
+  }
+
+  function {:opaque} FinishLoadingSuperblockPhase(k: Constants, cm: CM) : (cm' : CM)
+  requires cm.status.StatusLoadingSuperblock?
+  requires cm.superblock1.SuperblockSuccess?
+  requires cm.superblock2.SuperblockSuccess?
+  {
+    var idx := if JournalCache.increments1(
+        cm.superblock1.value.counter, cm.superblock2.value.counter)
+        then 1 else 0;
+
+    var sup := if idx == 1 then
+      cm.superblock2.value
+    else
+      cm.superblock1.value;
+
+    cm.(whichSuperblock := idx)
+      .(superblock := sup)
+      .(status := StatusLoadingOther)
+      .(journalFrontRead := None)
+      .(journalBackRead := None)
+  }
+
+  lemma FinishLoadingSuperblockPhaseCorrect(k: Constants, cm: CM)
+  requires cm.status.StatusLoadingSuperblock?
+  requires cm.superblock1.SuperblockSuccess?
+  requires cm.superblock2.SuperblockSuccess?
+  requires CommitterModel.WF(cm)
+  ensures var cm' := FinishLoadingSuperblockPhase(k, cm);
+    && CommitterModel.WF(cm')
+    && JournalCache.Next(Ik(k).jc,
+        CommitterModel.I(cm),
+        CommitterModel.I(cm'),
+        JournalDisk.NoDiskOp,
+        SendPersistentLocOp(cm'.superblock.indirectionTableLoc))
+  {
+    var cm' := FinishLoadingSuperblockPhase(k, cm);
+    var vop := SendPersistentLocOp(cm'.superblock.indirectionTableLoc);
+    reveal_FinishLoadingSuperblockPhase();
+    assert JournalCache.FinishLoadingSuperblockPhase(Ik(k).jc,
+        CommitterModel.I(cm),
+        CommitterModel.I(cm'),
+        JournalDisk.NoDiskOp,
+        vop);
+    assert JournalCache.NextStep(Ik(k).jc,
+        CommitterModel.I(cm),
+        CommitterModel.I(cm'),
+        JournalDisk.NoDiskOp,
+        vop,
+        JournalCache.FinishLoadingSuperblockPhaseStep);
+  }
+
+  function {:opaque} FinishLoadingOtherPhase(k: Constants, cm: CM) : (cm' : CM)
+  requires cm.status.StatusLoadingOther?
+  requires CommitterModel.WF(cm)
+  {
+    if cm.superblock.journalLen == 0 then
+      cm.(status := StatusReady)
+        .(frozenLoc := None)
+        .(isFrozen := false)
+        .(frozenJournalPosition := 0)
+        .(superblockWrite := None)
+        .(outstandingJournalWrites := {})
+        .(newSuperblock := None)
+        .(commitStatus := JournalCache.CommitNone)
+        .(journalist := JournalistModel.setWrittenJournalLen(
+            cm.journalist, cm.superblock.journalLen))
+    else
+      cm
+  }
+
+  lemma FinishLoadingOtherPhaseCorrect(k: Constants, cm: CM)
+  requires cm.status.StatusLoadingOther?
+  requires CommitterModel.WF(cm)
+  ensures var cm' := FinishLoadingOtherPhase(k, cm)
+  {
+  }
 }
